Logic/Modal/Normal/New/Completeness.lean
@@ -1,0 +1,6 @@
+import Logic.Modal.Normal.New.Kripke
+import Logic.Modal.Normal.New.Hilbert
+
+namespace LO.Modal.Normal.Kripkean
+
+end LO.Modal.Normal.Kripkean
