Logic/Modal/Normal/New/Soundness.lean
@@ -4,30 +4,46 @@ import Logic.Modal.Normal.New.Hilbert
 namespace LO.Modal.Normal.Kripkean
 
 variable {W α : Type*}
+variable {Λ : AxiomSet α}
 
+open Deduction
 open Formula.Kripkean
 
-instance {Λ : AxiomSet α} : Sound Λ (𝔽(Λ) : FrameClass W α) where
-  sound d := by
-    induction d.some with
-    | maxm h => intro F hF; exact hF.realize h;
-    | mdp hpq hp ihpq ihp =>
-      intro F hF V w;
-      have := (ihpq ⟨hpq⟩) F hF V w;
-      have := (ihp ⟨hp⟩) F hF V w;
-      simp_all;
-    | nec h ih =>
-      intro F hF V w w' _;
-      have := (ih ⟨h⟩) F hF V w';
-      simp_all;
-    | disj₃ =>
-      simp_all [ValidOnFrameClass, ValidOnFrame, ValidOnModel];
-      intros; rename_i hpr hqr hpq;
-      cases hpq with
-      | inl hp => exact hpr hp;
-      | inr hq => exact hqr hq;
-    | _ => simp_all [ValidOnFrameClass, ValidOnFrame, ValidOnModel];
+lemma sound (d : Λ ⊢ p) : (𝔽 : AxiomSetFrameClass W Λ) ⊧ p := by
+  induction d with
+  | maxm h => exact validOnAxiomSetFrameClass_axiom h;
+  | mdp _ _ ihpq ihp =>
+    intro F hF V w;
+    have := ihpq F hF V w;
+    have := ihp F hF V w;
+    simp_all;
+  | nec _ ih =>
+    intro F hF V w w' _;
+    have := ih F hF V w';
+    simp_all;
+  | disj₃ =>
+    simp_all [ValidOnAxiomSetFrameClass, ValidOnFrameClass, ValidOnFrame, ValidOnModel];
+    intros; rename_i hpr hqr hpq;
+    cases hpq with
+    | inl hp => exact hpr hp;
+    | inr hq => exact hqr hq;
+  | _ => simp_all [ValidOnAxiomSetFrameClass, ValidOnFrameClass, ValidOnFrame, ValidOnModel];
 
-instance : Sound 𝐊 (𝔽(𝐊) : FrameClass W α) := inferInstance
+lemma sound! : Λ ⊢! p → (𝔽Λ : AxiomSetFrameClass W Λ) ⊧ p := λ ⟨d⟩ => sound d
+
+instance : Sound Λ (𝔽Λ : AxiomSetFrameClass W Λ) := ⟨sound!⟩
+
+/-
+theorem soundness {T : Theory α} {p : Formula α} : T ⊢[Λ] p → T ⊨[AxiomSetFrameClass W Λ] p := by
+  intro ⟨Γ, hΓ, d⟩ 𝔽 h𝔽;
+  by_contra hC;
+  simp [ValidOnAxiomSetFrameClass, ValidOnFrameClass] at hC;
+  obtain ⟨F, ⟨hF, V⟩⟩ := hC;
+  simp [Semantics.models] at h𝔽;
+  intro F hF V w;
+  have := 𝔽.spec.mp hF;
+
+theorem soundness! {T : Theory α} {p} : T ⊢! p → T ⊨[AxiomSetFrameClass W Λ] p := λ ⟨d⟩ => soundness d
+-/
 
 end LO.Modal.Normal.Kripkean
